Util/Multiset/MultisetNat.v
@@ -9,6 +9,7 @@ multisets of natural numbers
 
 Set Implicit Arguments.
 
+Require Import Arith.
 Require Import MultisetTheory.
 Require Import MultisetOrder.
 Require Import MultisetList.
@@ -18,14 +19,26 @@ Module Nat.
   Definition A := nat.
 End Nat.
 
-Module Eqset := Eqset_def Nat.
+Module NatSet <: Eqset := Eqset_def Nat.
 
-Module MSetCore := MultisetList.MultisetList Eqset.
+Module NatSet_dec.
+
+  Module Eq := NatSet.
+  Export Eq.
+
+  Definition eqA_dec := eq_nat_dec.
+
+End NatSet_dec.
+
+Module MSetCore := MultisetList.MultisetList NatSet_dec.
 
 Module MSetTheory := MultisetTheory.Multiset MSetCore.
-
+ (* FIXME, the notation below is introduced only because otherwise 
+    doing 'Export LMO' results in an error: "Scope sets_scope is not
+    declared". This, I believe, should not be the case and maybe is
+    a temporary flaw of the development version of Coq 8.2. *)
+Notation "'XXX'" := I : sets_scope.
 Export MSetTheory.
 
 Module MSetOrd := MultisetOrder.MultisetOrder MSetCore.
-
 Export MSetOrd.
